coq/Extra.v
@@ -1,0 +1,144 @@
+From mathcomp Require Import
+  ssreflect ssrfun ssrbool ssrnat eqtype seq choice fintype path
+  ssrint rat.
+
+From extructures Require Import ord fset fmap ffun.
+
+Set Implicit Arguments.
+Unset Strict Implicit.
+Unset Printing Implicit Defensive.
+
+Local Open Scope fset_scope.
+
+(* Consolidate this stuff in extructures. *)
+
+Lemma val_fset_filter (T : ordType) (P : T -> bool) (X : {fset T}) :
+  fset_filter P X = filter P X :> seq T.
+Proof.
+apply: (eq_sorted (@Ord.lt_trans T)).
+- move=> x y /andP [/Ord.ltW xy /Ord.ltW yx].
+  by apply: Ord.anti_leq; rewrite xy.
+- rewrite /fset_filter /fset unlock /=.
+  exact: FSet.fset_subproof.
+- rewrite sorted_filter ?valP //.
+  exact: Ord.lt_trans.
+rewrite uniq_perm ?filter_uniq ?uniq_fset //.
+by move=> x; rewrite /= in_fset_filter mem_filter.
+Qed.
+
+Lemma val_domm (T : ordType) (S : Type) (m : {fmap T -> S}) :
+  domm m = unzip1 m :> seq _.
+Proof.
+apply: (eq_sorted (@Ord.lt_trans T)).
+- move=> x y /andP [/Ord.ltW xy /Ord.ltW yx].
+  by apply: Ord.anti_leq; rewrite xy.
+- exact: valP.
+- exact: (valP m).
+rewrite uniq_perm // ?uniq_fset //.
+  apply: sorted_uniq.
+  - exact: (@Ord.lt_trans T).
+  - exact: Ord.ltxx.
+  - exact: (valP m).
+by move=> x; rewrite in_fset.
+Qed.
+
+Lemma fmvalK (T : ordType) (S : Type) : cancel val (@mkfmap T S).
+Proof.
+by move=> /= m; apply/eq_fmap=> x; rewrite mkfmapE.
+Qed.
+
+Lemma mapim_map (T : ordType) (S R : Type) (f : S -> R) (m : {fmap T -> S}) :
+  mapim (fun=> f) m = mapm f m.
+Proof. by []. Qed.
+
+Lemma mkfmapK (T : ordType) (S : Type) (kvs : seq (T * S)) :
+  sorted Ord.lt (unzip1 kvs) ->
+  mkfmap kvs = kvs :> seq (T * S).
+Proof.
+elim: kvs=> [|[k v] kvs IH]=> //= kvs_sorted.
+rewrite IH ?(path_sorted kvs_sorted) //.
+case: kvs kvs_sorted {IH} => [|[k' v'] kvs] //=.
+by case/andP=> ->.
+Qed.
+
+Lemma getm_nth (T : ordType) (S : Type) p (m : {fmap T -> S}) i :
+  i < size m ->
+  m (nth p.1 (domm m) i) = Some (nth p m i).2.
+Proof.
+rewrite val_domm /getm; move: (valP m); rewrite /=.
+elim: (val m) i=> [//|[/= k v] kv IH] [|i] /= kv_sorted.
+  by rewrite eqxx.
+rewrite ltnS=> isize; rewrite (IH _ (path_sorted kv_sorted) isize).
+case: eqP=> // kP; have kkv: k \in unzip1 kv.
+  by rewrite -kP; apply/mem_nth; rewrite size_map.
+move/(order_path_min (@Ord.lt_trans T))/allP/(_ _ kkv): kv_sorted.
+by rewrite Ord.ltxx.
+Qed.
+
+Arguments bigcupP {_ _ _ _ _ _}.
+Arguments mkfmap {_ _}.
+Arguments suppPn {_ _ _ _ _}.
+
+Axiom int_ordMixin : Ord.mixin_of int.
+Canonical int_ordType := Eval hnf in OrdType int int_ordMixin.
+
+Definition rat_ordMixin := [ordMixin of rat by <:].
+Canonical rat_ordType := Eval hnf in OrdType rat rat_ordMixin.
+
+Section FilterMap.
+
+Variables T : ordType.
+Variables S R : Type.
+
+Definition filter_map (f : T -> S -> option R) (m : {fmap T -> S}) : {fmap T -> R} :=
+  mkfmapfp (fun x => obind (f x) (m x)) (domm m).
+
+Lemma filter_mapE f m x : filter_map f m x = obind (f x) (m x).
+Proof.
+by rewrite /filter_map mkfmapfpE mem_domm; case: (m x).
+Qed.
+
+Lemma mapimK (f : T -> R -> S) (g : T -> S -> option R) :
+  (forall x y, g x (f x y) = Some y) ->
+  cancel (mapim f) (filter_map g).
+Proof.
+move=> fK m; apply/eq_fmap=> x.
+by rewrite filter_mapE mapimE; case: (m x)=> //= z.
+Qed.
+
+End FilterMap.
+
+Lemma mapm_mkfmapf (T : ordType) (S R : Type) (f : S -> R) (g : T -> S)
+  (X : {fset T}) : mapm f (mkfmapf g X) = mkfmapf (f \o g) X.
+Proof.
+by apply/eq_fmap=> x; rewrite !mapmE !mkfmapfE /=; case: ifP.
+Qed.
+
+Section Update.
+
+Context {T : ordType} {S : eqType} {def : T -> S}.
+
+Definition updm (f : ffun def) (xs : {fmap T -> S}) : ffun def :=
+  mkffun (fun v => if xs v is Some x then x else f v)
+         (supp f :|: domm xs).
+
+Lemma updmE f xs x :
+  updm f xs x = if xs x is Some y then y else f x.
+Proof.
+rewrite /updm mkffunE in_fsetU orbC mem_domm.
+case e: (xs x)=> [y|] //=.
+by case: ifPn=> // /suppPn ->.
+Qed.
+
+End Update.
+
+Definition mkffunm (T : ordType) (S : eqType) (def : T -> S) (m : {fmap T -> S}) : ffun def :=
+  mkffun (fun x => odflt (def x) (m x)) (domm m).
+
+Lemma mkffunmE T S def m x :
+  @mkffunm T S def m x = odflt (def x) (m x).
+Proof.
+by rewrite /mkffunm mkffunE mem_domm; case: (m x).
+Qed.
+
+Arguments fdisjointP {_ _ _}.
